Made classical like the good old days.

HOL/ClassicalProofScript.sml
@@ -10,59 +10,79 @@ open bagTheory;
 open pred_setTheory;
 
 open FormulaSyntaxTheory;
-open BagLemmataTheory;
 
 val _ = new_theory "ClassicalProof";
 
 (** Natural Deduction for classical logic **)
-(* Nc is the 'deduciblility' relation for this system *)
+(* N is the 'deduciblility' relation for this system *)
 (* A, B and C are used to represent formulae *)
 (* D, D1, D2, D3 are used to represent the set of open assumptions *)
 (* I'm representing the deductions simply with unlabeled sets of
    open assumptions, as in T&S 2.1.8-2.1.9 (p.41--44) *)
 
-val _ = set_fixity "Nc" (Infix(NONASSOC,320));
-val _ = set_fixity "Gc" (Infix(NONASSOC,320));
+val (N_rules, N_ind, N_cases) = Hol_reln `
+(! (A :'a formula). N {A} A) (* Base case *)
+/\ (!A B D1 D2. (N D1 A) /\ (N D2 B)
+   ==> (N (D1 UNION D2) (A And B))) (* And Intro *)
+/\ (!A B D. (N D (A And B)) ==> N D A) (* And Elimination Left Conjunct *)
+/\ (!A B D. (N D (A And B)) ==> N D B) (* And Elim Right Conjunct *)
+/\ (!A B D. (N (A INSERT D) B) ==> N D (A Imp B)) (* Imp Intro *)
+/\ (!A B D1 D2. (N D1 (A Imp B)) /\ (N D2 A)
+   ==> N (D1 UNION D2) B) (* Imp Elim *)
+/\ (!A B D. N D A ==> N D (A Or B))  (* Or Intro right *)
+/\ (!A B D. N D B ==> N D (A Or B))  (* Or Intro left *)
+/\ (!A B C D D1 D2. (N D (A Or B)) /\ (* Or Elim *)
+(N (A INSERT D1) C) /\ (N (B INSERT D2) C) ==> N (D ∪ D1 ∪ D2) C)
+/\ (!A D. (N ((Not A) INSERT D) Bot) ==> (N D A))`; (* Classical Absurdity Rule *)
 
-val (Nc_rules, Nc_ind, Nc_cases) = Hol_reln `
-(! (A :'a formula). {A} Nc A) (* Base case *)
-/\ (!A B D1 D2 D. (D1 Nc A) /\ (D2 Nc B)
-   /\ (D = (D1 UNION D2)) ==> D Nc (A And B)) (* And Intro *)
-/\ (!A B D. (D Nc (A And B)) ==> D Nc A) (* And Elimination Left Conjunct *)
-/\ (!A B D. (D Nc (A And B)) ==> D Nc B) (* And Elim Right Conjunct *)
-/\ (!A B D. ((A INSERT D) Nc B) ==> D Nc (A Imp B)) (* Imp Intro *)
-/\ (!A B D1 D2 D. (D1 Nc (A Imp B)) /\ (D2 Nc A) /\ (D = (D1 UNION D2))
-    ==> D Nc B) (* Imp Elim *)
-/\ (!A B D. D Nc A ==> D Nc (A Or B))  (* Or Intro right *)
-/\ (!A B D. D Nc B ==> D Nc (A Or B))  (* Or Intro left *)
-/\ (!A B C D D1 D2 D0. (D Nc (A Or B)) /\ (* Or Elim *)
-    ((A INSERT D1) Nc C) /\ ((B INSERT D2) Nc C) /\ (D0 = (D ∪ D1 ∪ D2))
-    ==> D0 Nc C)
-/\ (!A D. (((Not A) INSERT D) Nc Bot) (* Classical Absurdity Rule *)
-==> (D Nc A))`; 
+val [N_ax, N_andi, N_andel, N_ander,
+     N_impi, N_impe, N_orir, N_oril, N_ore, N_bot] = CONJUNCTS N_rules;
 
-val [Nc_ax, Nc_andi, Nc_andel, Nc_ander,
-     Nc_impi, Nc_impe, Nc_orir, Nc_oril, Nc_ore, Nc_bot] = CONJUNCTS Nc_rules;
-
-Theorem Nc_FINITE:
-  !D A. D Nc A ==> FINITE D
-Proof
-  Induct_on `D Nc A` >> 
-  rw[]
+Theorem N_FINITE:
+  !D A. N D A ==> FINITE D
+Proof Induct_on `N` >> rw[]
 QED
 
-Theorem Nc_lw:
-  ∀D A. D Nc A ==> ∀B. (B INSERT D) Nc A
+val (Nd_rules, Nd_ind, Nd_cases) = Hol_reln `
+(! (A :'a formula). Nd {A} A) (* Base case *)
+/\ (!A B D1 D2. (Nd D1 A) /\ (Nd D2 B)
+    ==> (Nd (D1 UNION D2) (A And B))) (* And Intro *)
+/\ (!A B D. (Nd D (A And B)) ==> Nd D A) (* And Elimination Left Conjunct *)
+/\ (!A B D. (Nd D (A And B)) ==> Nd D B) (* And Elim Right Conjunct *)
+/\ (!A B D. (Nd D B) ==> Nd (D DELETE A) (A Imp B)) (* Imp Intro *)
+/\ (!A B D1 D2. (Nd D1 (A Imp B)) /\ (Nd D2 A)
+    ==> Nd (D1 UNION D2) B) (* Imp Elim *)
+/\ (!A B D. Nd D A ==> Nd D (A Or B)) (* Or Intro right *)
+/\ (!A B D. Nd D B ==> Nd D (A Or B)) (* Or Intro left *)
+/\ (!A B C D D1 D2. (Nd D (A Or B)) /\ (Nd D1 C) /\ (Nd D2 C)
+    ==> Nd (D ∪ (D1 DELETE A) ∪ (D2 DELETE B)) C) (* Or Elim *)
+/\ (!A D. (Nd D Bot) ==> (Nd (D DELETE (Not A)) A))`; (* Classical Absurdity Rule *)
+
+val [Nd_ax, Nd_andi, Nd_andel, Nd_ander,
+     Nd_impi, Nd_impe, Nd_orir, Nd_oril, Nd_ore, Nd_bot] = CONJUNCTS Nd_rules;
+
+Theorem N_lw:
+  ∀D A. N D A ==> ∀B. N (B INSERT D) A
 Proof
   rw[] >>
-  `{B} Nc B` by metis_tac[Nc_ax] >>
-  `({B} ∪ D) Nc (B And A)` by metis_tac[Nc_andi] >>
-  `({B} ∪ D) Nc A` by metis_tac[Nc_ander] >>
+  `N {B} B` by metis_tac[N_ax] >>
+  `N ({B} ∪ D) (B And A)` by metis_tac[N_andi] >>
+  `N ({B} ∪ D) A` by metis_tac[N_ander] >>
   metis_tac[INSERT_SING_UNION]
 QED
 
-Theorem Nc_lw_SUBSET:
-  ∀D'. FINITE D' ==> ∀D A. (D Nc A) /\ D ⊆ D' ==> D' Nc A
+Theorem Nd_lw:
+∀D A. Nd D A ==> ∀B. Nd (B INSERT D) A
+Proof
+  rw[] >>
+  `Nd {B} B` by metis_tac[Nd_ax] >>
+  `Nd ({B} ∪ D) (B And A)` by metis_tac[Nd_andi] >>
+  `Nd ({B} ∪ D) A` by metis_tac[Nd_ander] >>
+  metis_tac[INSERT_SING_UNION]
+QED
+
+Theorem N_lw_SUBSET:
+  ∀D'. FINITE D' ==> ∀D A. N D A  /\ D ⊆ D' ==> N D' A
 Proof
   GEN_TAC >>
   Induct_on `CARD D'`
@@ -73,21 +93,40 @@ Proof
       >- metis_tac[]
       >- (`?D₀ e. (D' = e INSERT D₀) /\ D ⊆ D₀ /\ e NOTIN D₀`
             by (`?e. e ∈ D' /\ e NOTIN D`
-              by metis_tac[PSUBSET_DEF,PSUBSET_MEMBER] >>
-              qexists_tac `D' DELETE e` >>
-              qexists_tac `e` >>
-              simp[] >>
-              fs[SUBSET_DEF]) >>
+            by metis_tac[PSUBSET_DEF,PSUBSET_MEMBER] >>
+            qexists_tac `D' DELETE e` >>
+            qexists_tac `e` >>
+            simp[] >>
+            fs[SUBSET_DEF]) >>
           rw[] >>
           fs[] >>
-          metis_tac[Nc_lw]))
+          metis_tac[N_lw]))
 QED
 
-Theorem Nc_impi_DELETE:
-  ∀D A B. D Nc A ==> (D DELETE B) Nc (B Imp A)
+Theorem Nd_lw_SUBSET:
+∀D'. FINITE D' ==> ∀D A. Nd D A  /\ D ⊆ D' ==> Nd D' A
+Proof
+  GEN_TAC >>
+  Induct_on `CARD D'`
+  >- (rw[] >> metis_tac[CARD_EQ_0,SUBSET_EMPTY])
+  >- (rw[] >> Cases_on `D=D'` >- metis_tac[] >>
+      `?D₀ e. (D' = e INSERT D₀) /\ D ⊆ D₀ /\ e NOTIN D₀`
+        by (`?e. e ∈ D' /\ e NOTIN D`
+              by metis_tac[PSUBSET_DEF,PSUBSET_MEMBER] >>
+            qexists_tac `D' DELETE e` >>
+            qexists_tac `e` >>
+            simp[] >>
+            fs[SUBSET_DEF]) >>
+      rw[] >>
+      fs[] >>
+      metis_tac[Nd_lw])
+QED
+
+Theorem N_impi_DELETE:
+  ∀D A B. N D A ==> N (D DELETE B) (B Imp A)
 Proof
   rw[] >>
-  `(B INSERT D) Nc A` by metis_tac[Nc_lw] >>
+  `N (B INSERT D) A` by metis_tac[N_lw] >>
   Cases_on `B ∈ D`
     >- (`?D'. (D = B INSERT D') /\ B NOTIN D'`
           by metis_tac[DECOMPOSITION] >>
@@ -95,403 +134,312 @@ Proof
         `(B INSERT D') DELETE B = D'`
           by (dsimp[EXTENSION] >>
               metis_tac[]) >>
-        simp[Nc_impi])
-    >- simp[DELETE_NON_ELEMENT_RWT,Nc_impi]
+        simp[N_impi])
+    >- simp[DELETE_NON_ELEMENT_RWT,N_impi]
 QED
 
-val NcThm = Define `NcThm A = EMPTY Nc A`;
+Theorem N_Nd:
+  ∀D A. N D A <=> Nd D A
+Proof
+ `(∀D A:'a formula. N D A ==> Nd D A) ∧
+  (∀D A:'a formula. Nd D A ==> N D A)`
+    suffices_by metis_tac[] >>
+  conj_tac
+  >- (Induct_on `N` >>
+      rw[Nd_rules]
+        >- metis_tac[Nd_andel]
+        >- metis_tac[Nd_ander]
+        >- (`Nd ((A INSERT D) DELETE A) (A Imp B)`
+              by metis_tac[Nd_impi] >>
+            Cases_on `A ∈ D`
+              >- (fs[DELETE_DEF] >>
+                  `Nd (A INSERT (D DIFF {A})) (A Imp B)`
+                    by metis_tac[Nd_lw] >>
+                  fs[Once INSERT_SING_UNION] >>
+                  `{A} ⊆ D` by simp[SUBSET_DEF] >>
+                  metis_tac[UNION_DIFF])
+              >- fs[DELETE_DEF,DELETE_NON_ELEMENT])
+        >- metis_tac[Nd_impe]
+        >- (`Nd (D ∪ ((A INSERT D1) DELETE A) ∪ ((B INSERT D2) DELETE B)) C`
+              by metis_tac[Nd_ore] >>
+            fs[DELETE_DEF] >>
+            irule Nd_lw_SUBSET >>
+            `FINITE (D ∪ D1 ∪ D2)`
+              by (simp[FINITE_UNION] >> metis_tac[N_FINITE,FINITE_INSERT]) >>
+            simp[] >>
+            qexists_tac `D ∪ (D1 DIFF {A}) ∪ (D2 DIFF {B})` >>
+            rw[SUBSET_DEF])
+        >- (`Nd ((Not A INSERT D) DELETE Not A) A` by metis_tac[Nd_bot] >>
+            fs[DELETE_DEF] >>
+            irule Nd_lw_SUBSET >>
+            conj_tac >- metis_tac[N_FINITE,FINITE_INSERT] >>
+            metis_tac[DIFF_SUBSET]))
+  >- (Induct_on `Nd` >>
+      rw[N_rules]
+        >- metis_tac[N_andel]
+        >- metis_tac[N_ander]
+        >- metis_tac[N_impi_DELETE]
+        >- metis_tac[N_impe]
+        >- (`N (A INSERT (D1 DELETE A)) C`
+              by (irule N_lw_SUBSET >>
+                  rw[] >- metis_tac[N_FINITE] >>
+                  qexists_tac `D1` >>
+                  rw[DELETE_DEF,SUBSET_DEF]) >>
+            `N (B INSERT (D2 DELETE B)) C`
+              by (irule N_lw_SUBSET >>
+                  rw[] >- metis_tac[N_FINITE] >>
+                  qexists_tac `D2` >>
+                  rw[DELETE_DEF,SUBSET_DEF]) >>
+            metis_tac[N_ore])
+        >- (`N (Not A INSERT D) Bot` by metis_tac[N_lw] >>
+            irule N_bot >>
+            Cases_on `Not A ∈ D`
+              >- (`?D'. (D = Not A INSERT D') /\ Not A NOTIN D'` 
+                    by metis_tac[DECOMPOSITION] >>
+                  fs[] >> rw[])
+              >- fs[DELETE_NON_ELEMENT_RWT]))
+QED
+
+val NThm = Define `NThm A = N EMPTY A`;
 
 (* Example deductions *)
-val Nc_example = Q.prove(`NcThm (A Imp (B Imp A))`,
-`{A} Nc A` by rw[Nc_ax] >>
-`{B} Nc B` by rw[Nc_ax] >>
+val N_example = Q.prove(`NThm (A Imp (B Imp A))`,
+`N {A} A` by rw[N_ax] >>
+`N {B} B` by rw[N_ax] >>
 `{A} UNION {B} = {A;B}` by simp[UNION_DEF,INSERT_DEF] >>
-`{A;B} Nc (A And B)` by metis_tac[Nc_andi] >>
-`{A;B} Nc (A)` by metis_tac[Nc_andel] >>
-`{A} Nc (B Imp A)` by (irule Nc_impi >> simp[INSERT_COMM]) >>
-`{} Nc (A Imp (B Imp A))` by metis_tac[Nc_impi] >>
- rw[NcThm]);
+`N {A;B} (A And B)` by metis_tac[N_andi] >>
+`N {A;B} (A)` by metis_tac[N_andel] >>
+`N {A} (B Imp A)` by (irule N_impi >> simp[INSERT_COMM]) >>
+`N {} (A Imp (B Imp A))` by metis_tac[N_impi] >>
+ rw[NThm]);
 
-val Nc_example = Q.prove(`NcThm (Bot Imp A)`,
-  `{Bot} Nc Bot` by rw[Nc_ax] >>
-  `{Not A;Bot} Nc Bot` by metis_tac[Nc_lw] >>
-  `{Bot} Nc A` by rw[Nc_bot] >>
-  `EMPTY Nc (Bot Imp A)` by metis_tac[Nc_rules,DIFF_DEF] >>
-  rw[NcThm]);
+(* val N_example = Q.prove(`NThm (Bot Imp A)`, *)
+(*   `N {Bot} Bot` by rw[N_rules] >> *)
+(*   `N {Bot} A` by rw[N_rules] >> *)
+(*   `{} = ({Bot} DIFF {Bot})` by rw[DIFF_DEF] >> *)
+(*   `N EMPTY (Bot Imp A)` by metis_tac[N_rules] >> *)
+(*   rw[NThm]); *)
 
 
 (** Sequent Calculus (Gentzen System) for classical logic **)
-(* Gc is the 'deduciblility' relation for this system *)
+(* G is the 'deduciblility' relation for this system *)
 (* A, B and C are used to represent formulae *)
 (* S is used to represent the multiset of the Antecedent Context *)
-(* The consequent is a multiset of formula in the classical logic *)
+(* The consequent is always a single formula in the intuitionistic logic *)
 
-val (Gc_rules, Gc_ind, Gc_cases) = Hol_reln `
-(!(A:'a formula) Γ Δ.
-                   (A <: Γ) /\ FINITE_BAG Γ /\
-                   (A <: Δ) /\ FINITE_BAG Δ
-                   ==> Γ Gc Δ) (* Ax *)
-/\ (∀ Γ Δ. (Bot <: Γ) /\ FINITE_BAG Γ /\ FINITE_BAG Δ ==> Γ Gc Δ) (* LBot *)
-/\ (!A Γ Δ Σ. (({|A;A|} + Γ) Gc Δ) /\ (Σ = ({|A|} + Γ))
-                     ==> Σ Gc Δ) (* Left Contraction *)
-/\ (!A Γ Δ Σ. (Γ Gc ({|A;A|} + Δ)) /\ (Σ = ({|A|} + Δ))
-                     ==> Γ Gc Σ) (* Right Contraction *)
-/\ (!A B Γ Δ Σ. ((BAG_INSERT A Γ) Gc Δ)
-   /\ (Σ = (BAG_INSERT (A And B) Γ)) ==> Σ Gc Δ) (* Left And 1 *)
-/\ (!A B Γ Δ Σ. ((BAG_INSERT B Γ) Gc Δ)
-    /\ (Σ = (BAG_INSERT (A And B) Γ)) ==> Σ Gc Δ) (* Left And 1 *)
-/\ (!A B Γ Δ Σ. (Γ Gc (BAG_INSERT A Δ)) /\ (Γ Gc (BAG_INSERT B Δ))
-              /\ (Σ = BAG_INSERT (A And B) Δ)
-              ==> Γ Gc Σ) (* Right And *)
-/\ (!A B Γ Δ. ((BAG_INSERT A Γ) Gc Δ)
-    /\ ((BAG_INSERT B Γ) Gc Δ)
-    /\ (Σ = (BAG_INSERT (A Or B) Γ)) ==> Σ Gc Δ) (* Left Or *)
-/\ (!A B Γ Δ Δ'. (Γ Gc (BAG_INSERT A Δ)) /\ (Δ' = (BAG_INSERT (A Or B) Δ))
-   ==> Γ Gc Δ') (* Right Or 1 *)
-/\ (!A B Γ Δ Δ'. (Γ Gc (BAG_INSERT B Δ)) /\ (Δ' = (BAG_INSERT (A Or B) Δ))
-   ==> Γ Gc Δ') (* Right Or 2 *)
-/\ (!A B Γ Δ Σ. (Γ Gc (BAG_INSERT A Δ)) /\ ((BAG_INSERT B Γ) Gc Δ)
-              /\ (Σ = (BAG_INSERT (A Imp B) Γ)) ==> Σ Gc Δ) (* Left Imp *)
-/\ (!A B Γ Δ Δ'. ((BAG_INSERT A Γ) Gc (BAG_INSERT B Δ))
-                 /\ (Δ' = BAG_INSERT (A Imp B) Δ)
-                 ==> (Γ Gc Δ)) (* Right Imp *)
-/\ (∀A Γ Γ' Δ Δ'. (Γ Gc (BAG_INSERT A Δ)) ∧ ((BAG_INSERT A Γ') Gc Δ') 
-                       ==> Γ ⊎ Γ' Gc Δ ⊎ Δ')` (* Cut_cs *)
+val (G_rules, G_ind, G_cases) = Hol_reln `
+(!(A:'a formula) Γ Δ. (A <: Γ) /\ FINITE_BAG Γ /\
+                      (A <: Δ) /\ FINITE_BAG Δ
+                      ==> G Γ Δ) (* Ax *)
+/\ (∀ Γ Δ. (Bot <: Γ) /\ FINITE_BAG Γ /\ FINITE_BAG Δ ==> G Γ Δ) (* LBot *)
+/\ (!A Γ Δ. (G ({|A;A|} + Γ) Δ) ==> G ({|A|} + Γ) Δ) (* Left Contraction *)
+/\ (!A Γ Δ. (G Γ ({|A;A|} + Δ)) ==> G Γ ({|A|} + Δ)) (* Right Contraction *)
+/\ (!A B Γ Δ. (G (BAG_INSERT A Γ) Δ)
+   ==> (G (BAG_INSERT (A And B) Γ) Δ)) (* Left And 1 *)
+/\ (!A B Γ Δ. (G (BAG_INSERT B Γ) Δ)
+   ==> (G (BAG_INSERT (A And B) Γ) Δ)) (* Left And 2 *)
+/\ (!A B Γ Δ. (G Γ (BAG_INSERT A Δ)) /\ (G Γ (BAG_INSERT B Δ))
+    ==> G Γ (BAG_INSERT (A And B) Δ)) (* Right And *)
+/\ (!A B Γ Δ. (G (BAG_INSERT A Γ) Δ)
+    /\ (G (BAG_INSERT B Γ) Δ)
+    ==> G ((BAG_INSERT (A Or B) Γ)) Δ) (* Left Or *)
+/\ (!A B Γ Δ. (G Γ (BAG_INSERT A Δ))
+    ==> G Γ (BAG_INSERT (A Or B) Δ)) (* Right Or 1 *)
+/\ (!A B Γ Δ. (G Γ (BAG_INSERT B Δ)) 
+    ==> G Γ (BAG_INSERT (A Or B) Δ)) (* Right Or 2 *)
+/\ (!A B Γ Δ. (G Γ (BAG_INSERT A Δ)) /\ (G (BAG_INSERT B Γ) Δ)
+    ==> G Γ ((BAG_INSERT (A Imp B) Δ))) (* Left Imp *)
+/\ (!A B Γ Δ. (G (BAG_INSERT A Γ) (BAG_INSERT B Δ))
+    ==> G Γ (BAG_INSERT (A Imp B) Δ)) (* Right Imp *)
+/\ (∀A Γ Γ' Δ Δ'. (G Γ (BAG_INSERT A Δ)) ∧ (G (BAG_INSERT A Γ') Δ') 
+    ==> G (Γ ⊎ Γ') (Δ ⊎ Δ'))` (* Cut_cs *)
 
-val [Gc_ax, Gc_bot, Gc_lc, Gc_rc, Gc_landl, Gc_landr, Gc_rand,
-     Gc_lor, Gc_rorl, Gc_rorr, Gc_limp, Gc_rimp, Gc_cut] = CONJUNCTS Gc_rules;
-   
-(* val GcThm = Define `GcThm A = EMPTY_BAG Gc A`; *)
+val [G_ax, G_bot, G_lc, G_rc, G_landl, G_landr, G_rand,
+     G_lor, G_rorl, G_rorr, G_limp, G_rimp, G_cut] = CONJUNCTS G_rules;
 
-(* val Gc_example1 = *)
-(*     Q.prove(`GcThm ((A And B) Imp (B And A))`, rw[GcThm,Gc_rules]); *)
+val GThm = Define `GThm A = G EMPTY_BAG A`;
 
-(* val Gc_example2 = Q.prove (`GcThm ((A Imp (A Imp B)) Imp (A Imp B))`, *)
-(* rw[GcThm] >> *)
-(* `Gc {|(A Imp A Imp B)|} (A Imp B)` suffices_by metis_tac[Gc_rules] >> *)
-(* `Gc {|A;(A Imp A Imp B)|} (B)` suffices_by metis_tac[Gc_rules] >> *)
-(* `Gc {|A|} (A)` by metis_tac[Gc_ax,BAG_IN_BAG_INSERT,FINITE_BAG] >> *)
-(* `Gc {|B;A|} (B)` by metis_tac[Gc_ax,BAG_IN_BAG_INSERT,FINITE_BAG] >> *)
-(* (* `Gc {|A;B|} (B)` by simp[Gc_lw] >> *) *)
-(* (* `Gc {|B;A|} (B)` by simp[BAG_INSERT_commutes] >> *) *)
-(* `Gc {|(A Imp B);A|} (B)` by metis_tac[Gc_rules] >> *)
-(* `Gc {|(A Imp A Imp B);A|} (B)` suffices_by metis_tac[BAG_INSERT_commutes] >> *)
-(* metis_tac[Gc_rules]); *)
+(* val G_example1 = *)
+(*     Q.prove(`GThm ((A And B) Imp (B And A))`, rw[GThm,G_rules]); *)
 
-(* val Gc_land_commutes = *)
-(*     Q.prove(`Gc {| A And B |} Δ ==> Gc {| B And A |} Δ`, rw[] >> *)
-(* `Gc {|B|} B` by metis_tac[Gc_ax,BAG_IN_BAG_INSERT,FINITE_BAG] >> *)
-(* `Gc {|B And A|} B` by metis_tac[Gc_landl] >> *)
-(* `Gc {|A|} A` by metis_tac[Gc_ax,BAG_IN_BAG_INSERT,FINITE_BAG] >> *)
-(* `Gc {|B And A|} A` by metis_tac[Gc_landr] >> *)
-(* `Gc {|B And A|} (A And B)` by metis_tac[Gc_rand] >> *)
-(* `Gc ({|B And A|} + {||}) Δ` by metis_tac[Gc_cut] >> *)
+(* val G_example2 = Q.prove (`GThm ((A Imp (A Imp B)) Imp (A Imp B))`, *)
+(* rw[GThm] >> *)
+(* `G {|(A Imp A Imp B)|} (A Imp B)` suffices_by metis_tac[G_rules] >> *)
+(* `G {|A;(A Imp A Imp B)|} (B)` suffices_by metis_tac[G_rules] >> *)
+(* `G {|A|} (A)` by metis_tac[G_ax,BAG_IN_BAG_INSERT,FINITE_BAG] >> *)
+(* `G {|B;A|} (B)` by metis_tac[G_ax,BAG_IN_BAG_INSERT,FINITE_BAG] >> *)
+(* (* `G {|A;B|} (B)` by simp[G_lw] >> *) *)
+(* (* `G {|B;A|} (B)` by simp[BAG_INSERT_commutes] >> *) *)
+(* `G {|(A Imp B);A|} (B)` by metis_tac[G_rules] >> *)
+(* `G {|(A Imp A Imp B);A|} (B)` suffices_by metis_tac[BAG_INSERT_commutes] >> *)
+(* metis_tac[G_rules]); *)
+
+(* val G_land_commutes = *)
+(*     Q.prove(`G {| A And B |} Δ ==> G {| B And A |} Δ`, rw[] >> *)
+(* `G {|B|} B` by metis_tac[G_ax,BAG_IN_BAG_INSERT,FINITE_BAG] >> *)
+(* `G {|B And A|} B` by metis_tac[G_landl] >> *)
+(* `G {|A|} A` by metis_tac[G_ax,BAG_IN_BAG_INSERT,FINITE_BAG] >> *)
+(* `G {|B And A|} A` by metis_tac[G_landr] >> *)
+(* `G {|B And A|} (A And B)` by metis_tac[G_rand] >> *)
+(* `G ({|B And A|} + {||}) Δ` by metis_tac[G_cut] >> *)
 (* metis_tac[BAG_UNION_EMPTY]); *)
 
-Theorem Gc_FINITE:
-  !h c. h Gc c ==> FINITE_BAG h /\ FINITE_BAG c
-Proof
-  Induct_on `h Gc c` >> rw[]
+Theorem G_FINITE:
+  !Γ Δ. G Γ Δ ==> FINITE_BAG Γ /\ FINITE_BAG Δ
+Proof Induct_on `G` >> simp[]
 QED
 
-Theorem BAG_INSERT_SUB_BAG_DECOMPOSE:
-   !e b b'. BAG_INSERT e b <= b' ==> ?c. b' = BAG_INSERT e c
+(* Thanks for this theorem Michael *)
+Theorem G_lw:
+  ∀Γ A. G Γ A ⇒ ∀Γ'. Γ ≤ Γ' /\ FINITE_BAG Γ' ⇒ G Γ' A
+Proof
+  Induct_on `G` >> rw[]
+  >- metis_tac[G_ax,SUB_BAG, BAG_IN]
+  >- metis_tac[G_bot,SUB_BAG,BAG_IN]
+  >- (‘∃Γ₂. Γ' = {|A|} ⊎ Γ₂’
+        by (qexists_tac ‘Γ' - {|A|}’ >> irule SUB_BAG_DIFF_EQ >>
+            metis_tac[SUB_BAG_UNION_down]) >>
+      rw[] >> irule G_lc >> first_x_assum irule >> fs[])
+  >- metis_tac[G_rc,SUB_BAG,BAG_IN]
+  >- (‘∃Γ₂. Γ' = BAG_INSERT (A And B) Γ₂’
+        by (qexists_tac ‘Γ' - {|A And B|}’ >> fs[BAG_INSERT_UNION] >>
+            irule SUB_BAG_DIFF_EQ >> metis_tac[SUB_BAG_UNION_down]) >>
+      rw[] >> irule G_landl >> first_x_assum irule >> fs[SUB_BAG_INSERT])
+  >- (‘∃Γ₂. Γ' = BAG_INSERT (A And B) Γ₂’
+        by (qexists_tac ‘Γ' - {|A And B|}’ >> fs[BAG_INSERT_UNION] >>
+            irule SUB_BAG_DIFF_EQ >> metis_tac[SUB_BAG_UNION_down]) >>
+      rw[] >> irule G_landr >> first_x_assum irule >> fs[SUB_BAG_INSERT])
+  >- simp[G_rand]
+  >- (‘∃Γ₂. Γ' = BAG_INSERT (A Or B) Γ₂’
+        by (qexists_tac ‘Γ' - {|A Or B|}’ >> fs[BAG_INSERT_UNION] >>
+            irule SUB_BAG_DIFF_EQ >> metis_tac[SUB_BAG_UNION_down]) >>
+      rw[] >> fs[SUB_BAG_INSERT] >> irule G_lor >> conj_tac >>
+      first_x_assum (fn th => irule th >> fs[SUB_BAG_INSERT] >> NO_TAC))
+  >- simp[G_rorl]
+  >- simp[G_rorr]
+  >- (irule G_limp >> fs[SUB_BAG_INSERT])
+  >- simp[SUB_BAG_INSERT, G_rimp]
+  >- (rename [‘Γ₁ ⊎ Γ₂ ≤ Γ₃’] >>
+      ‘∃Γ₀. Γ₃ = Γ₀ ⊎ Γ₁ ⊎ Γ₂’
+        by metis_tac[SUB_BAG_EXISTS, COMM_BAG_UNION, ASSOC_BAG_UNION] >>
+      fs[] >> rw[] >> irule G_cut >>
+      qexists_tac ‘A’ >>
+      (* rename [‘G (BAG_INSERT A _) B’] >> *)
+      conj_tac >> first_x_assum irule >> fs[SUB_BAG_INSERT])
+QED
+
+Theorem G_lw_BAG_MERGE:
+  !Γ₁ A. G Γ₁ A ==> !Γ₂. FINITE_BAG Γ₂ ==> G (BAG_MERGE Γ₂ Γ₁) A
 Proof
   rw[] >>
-  irule BAG_DECOMPOSE >>
-  metis_tac[SUB_BAG_BAG_IN]
-QED
-
-Theorem EL_BAG_UNION_SUB_BAG_DECOMPOSE:
-  !e b b'. {|e|} + b <= b' ==> ?c. b' = BAG_INSERT e c
-Proof
-  rw[] >>
-  irule BAG_INSERT_SUB_BAG_DECOMPOSE >>
-  qexists_tac `b` >>
-  fs[BAG_INSERT_UNION]
-QED
-
-Theorem Gc_lw:
-  ∀Γ Δ. Γ Gc Δ ==> ∀Γ'. Γ ≤ Γ' /\ FINITE_BAG Γ' ==> Γ' Gc Δ
-Proof
-  Induct_on `Γ Gc Δ` >>
-  rw[]
-  >- (irule Gc_ax >> 
-      fs[] >> 
-      qexists_tac `A` >>
-      fs[SUB_BAG,BAG_IN])
-  >- (irule Gc_bot >> fs[SUB_BAG,BAG_IN])
-  >- (irule Gc_lc >>
-      qexists_tac `A` >>
-      `?b. Γ'' = BAG_INSERT A b`
-        by metis_tac[EL_BAG_UNION_SUB_BAG_DECOMPOSE] >>
-      fs[] >>
-      rw[] >>
-      qexists_tac `b` >>
-      simp[Once BAG_INSERT_UNION,EL_BAG] >>
-      first_x_assum (qspec_then `{|A;A|} ⊎ b` mp_tac) >>
-      fs[BAG_INSERT_UNION])
-  >- (irule Gc_rc >>
-      qexists_tac `A` >>
-      qexists_tac `Δ` >>
-      fs[])
-  >- (irule Gc_landl >>
-      qexists_tac `A` >>
-      qexists_tac `B` >>
-      `?b. Γ'' = BAG_INSERT (A And B) b`
-        by metis_tac[BAG_INSERT_SUB_BAG_DECOMPOSE] >>
-      fs[] >> rw[] >>
-      first_x_assum (qspec_then `BAG_INSERT A b` mp_tac) >>
-      fs[] >>
-      rw[SUB_BAG_INSERT] >>
-      `Γ ≤ b` suffices_by metis_tac[] >>
-      fs[SUB_BAG_INSERT])
-  >- (irule Gc_landr >>
-      qexists_tac `A` >>
-      qexists_tac `B` >>
-      `?b. Γ'' = BAG_INSERT (A And B) b`
-        by metis_tac[BAG_INSERT_SUB_BAG_DECOMPOSE] >>
-      fs[] >> rw[] >>
-      first_x_assum (qspec_then `BAG_INSERT B b` mp_tac) >>
-      fs[] >>
-      rw[SUB_BAG_INSERT] >>
-      `Γ ≤ b` suffices_by metis_tac[] >>
-      fs[SUB_BAG_INSERT])
-  >- (irule Gc_rand >> 
-      qexists_tac `A` >>
-      qexists_tac `B` >>
-      simp[])
-  >- (irule Gc_lor >>
-      qexists_tac `A` >>
-      qexists_tac `B` >>
-      `?b. Γ'' = BAG_INSERT (A Or B) b`
-        by metis_tac[BAG_INSERT_SUB_BAG_DECOMPOSE] >>
-      fs[] >> rw[] >>
-      first_x_assum (fn th => irule th >> fs[SUB_BAG_INSERT] >> NO_TAC))
-  >- (irule Gc_rorl >>
-      qexists_tac `A` >>
-      qexists_tac `B` >>
-      qexists_tac `Δ` >>
-      simp[])
-  >- (irule Gc_rorr >>
-            qexists_tac `A` >>
-            qexists_tac `B` >>
-            qexists_tac `Δ` >>
-            simp[])
-  >- (irule Gc_limp >> 
-      qexists_tac `A` >>
-      qexists_tac `B` >>
-      `?b. Γ'' = BAG_INSERT (A Imp B) b`
-        by metis_tac[BAG_INSERT_SUB_BAG_DECOMPOSE] >>
-        fs[] >> rw[] >>
-        first_x_assum (fn th => irule th >> fs[SUB_BAG_INSERT] >> NO_TAC))
-  >- (irule Gc_rimp >>
-      qexists_tac `A` >>
-      qexists_tac `B` >>
-      qexists_tac `BAG_INSERT (A Imp B) Δ` >>
-      simp[] >>
-      first_x_assum (fn th => irule th >> fs[SUB_BAG_INSERT] >> NO_TAC))
-  >- (
-      irule Gc_cut >>
-           
-      first_x_assum (qspec_then `BAG_INSERT A Γ'` mp_tac) >>
-      rw[] >>
-      fs[SUB_BAG_INSERT])
-QED
-
-Theorem Gc_rw:
-  ∀Γ Δ. Γ Gc Δ ==> ∀Δ'. Δ ≤ Δ' /\ FINITE_BAG Δ' ==> Γ Gc Δ'
-Proof
-  Induct_on `Γ Gc Δ` >>
-  rw[]
-  >- (irule Gc_ax >> 
-      fs[] >> 
-      qexists_tac `A` >>
-      fs[SUB_BAG,BAG_IN])
-  >- (irule Gc_bot >> fs[SUB_BAG,BAG_IN])
-  >- (irule Gc_lc >>
-      qexists_tac `A` >>
-      qexists_tac `Γ` >>
-      fs[])
-  >- (irule Gc_rc >>
-      qexists_tac `A` >>
-      `?b. Δ'' = BAG_INSERT A b`
-        by metis_tac[EL_BAG_UNION_SUB_BAG_DECOMPOSE] >>
-      fs[] >>
-      rw[] >>
-      qexists_tac `b` >>
-      simp[Once BAG_INSERT_UNION,EL_BAG] >>
-      first_x_assum (qspec_then `{|A;A|} ⊎ b` mp_tac) >>
-      fs[BAG_INSERT_UNION])
-  >- (irule Gc_landl >>
-      qexists_tac `A` >>
-      qexists_tac `B` >>
-      fs[])
-  >- (irule Gc_landr >>
-      qexists_tac `A` >>
-      qexists_tac `B` >>
-      fs[])
-  >- (irule Gc_rand >> 
-      qexists_tac `A` >>
-      qexists_tac `B` >>
-      `?b. Δ'' = BAG_INSERT (A And B) b`
-        by metis_tac[BAG_INSERT_SUB_BAG_DECOMPOSE] >>
-      fs[] >> rw[] >> 
-      first_x_assum (fn th => irule th >> fs[SUB_BAG_INSERT] >> NO_TAC))
-  >- (irule Gc_lor >>
-      qexists_tac `A` >>
-      qexists_tac `B` >>
-      qexists_tac `Γ'` >>
-      fs[])
-  >- (irule Gc_rorl >>
-      qexists_tac `A` >>
-      qexists_tac `B` >>
-      `?b. Δ'' = BAG_INSERT (A Or B) b`
-        by metis_tac[BAG_INSERT_SUB_BAG_DECOMPOSE] >>
-      fs[] >> rw[] >>
-      first_x_assum (fn th => irule th >> fs[SUB_BAG_INSERT] >> NO_TAC))
-  >- (irule Gc_rorr >>
-      qexists_tac `A` >>
-      qexists_tac `B` >>
-      `?b. Δ'' = BAG_INSERT (A Or B) b`
-        by metis_tac[BAG_INSERT_SUB_BAG_DECOMPOSE] >>
-      fs[] >> rw[] >>
-      first_x_assum (fn th => irule th >> fs[SUB_BAG_INSERT] >> NO_TAC))
-  >- (irule Gc_limp >> 
-      qexists_tac `A` >>
-      qexists_tac `B` >>
-      qexists_tac `Γ` >>
-      fs[] >>
-      first_x_assum (fn th => irule th >> fs[SUB_BAG_INSERT] >> NO_TAC))
-  >- (irule Gc_rimp >>
-      qexists_tac `A` >>
-      qexists_tac `B` >>
-      qexists_tac `BAG_INSERT (A Imp B) Δ''` >>
-      simp[] >>
-      first_x_assum (fn th => irule th >> fs[SUB_BAG_INSERT] >> NO_TAC))
-  >- (irule Gc_cut >>
-      qexists_tac `A` >>
-      first_x_assum (qspec_then `Δ'` mp_tac) >>
-      rw[] >>
-      first_x_assum (qspec_then `BAG_INSERT A Δ'` mp_tac) >>
-      rw[] >>
-      fs[SUB_BAG_INSERT])
-QED
-
-Theorem Gc_lw_BAG_MERGE:
-  !Γ₁ A. Γ₁ Gc A ==> !Γ₂. FINITE_BAG Γ₂ ==> (BAG_MERGE Γ₂ Γ₁) Gc A
-Proof
-  rw[] >>
-  irule Gc_lw >>
-  `FINITE_BAG Γ₁` by metis_tac[Gc_FINITE] >>
+  irule G_lw >>
+  `FINITE_BAG Γ₁` by metis_tac[G_FINITE] >>
   simp[FINITE_BAG_MERGE] >>
   qexists_tac `Γ₁` >>
   simp[SUB_BAG,BAG_INN_BAG_MERGE]
 QED
 
-Theorem Gc_lw_BAG_UNION:
-  ∀Γ A. (Γ Gc A) ==> ∀Γ'. FINITE_BAG Γ' ==> (Γ ⊎ Γ') Gc A
+Theorem G_lw_BAG_UNION:
+  ∀Γ A. G Γ A ==> ∀Γ'. FINITE_BAG Γ' ==> G (Γ ⊎ Γ') A
 Proof
   rw[] >>
-  irule Gc_lw >>
-  `FINITE_BAG Γ` by metis_tac[Gc_FINITE] >>
+  irule G_lw >>
+  `FINITE_BAG Γ` by metis_tac[G_FINITE] >>
   simp[FINITE_BAG_UNION] >>
   qexists_tac `Γ` >>
   simp[]
 QED
 
-Theorem Gc_rw_BAG_UNION:
-  ∀Γ Δ. (Γ Gc Δ) ==> !Δ'. FINITE_BAG Δ' ==> Γ Gc (Δ ⊎ Δ')
+Theorem G_lw_BAG_INSERT:
+  ∀Γ A. G Γ A ==> ∀B Γ'. G (BAG_INSERT B Γ) A
 Proof
   rw[] >>
-  irule Gc_rw >>
-  `FINITE_BAG Δ` by metis_tac[Gc_FINITE] >>
-  simp[FINITE_BAG_UNION] >>
-  qexists_tac `Δ` >>
-  simp[]
-QED
-
-Theorem Gc_lw_BAG_INSERT:
-  ∀Γ A. Γ Gc A ==> ∀B. (BAG_INSERT B Γ) Gc A
-Proof
-  rw[] >>
-  irule Gc_lw >>
-  `FINITE_BAG Γ` by metis_tac[Gc_FINITE] >>
+  irule G_lw >>
+  `FINITE_BAG Γ` by metis_tac[G_FINITE] >>
   simp[FINITE_BAG_THM] >>
   qexists_tac `Γ` >>
   simp[SUB_BAG_INSERT_I]
 QED
 
-Theorem Gc_rw_BAG_INSERT:
-  ∀Γ Δ. Γ Gc Δ ==> ∀B. Γ Gc (BAG_INSERT B Δ)
+Theorem G_rw:
+  ∀Γ Δ. G Γ Δ ==> ∀Δ'. Δ ≤ Δ' /\ FINITE_BAG Δ' ==> G Γ Δ'
 Proof
-  rw[] >>
-  irule Gc_rw >>
-  `FINITE_BAG Δ` by metis_tac[Gc_FINITE] >>
-  simp[FINITE_BAG_THM] >>
-  qexists_tac `Δ` >>
-  simp[SUB_BAG_INSERT_I]
+  Induct_on `G` >>
+  rw[G_rules]
+  >- metis_tac[G_ax,SUB_BAG,BAG_IN]
+  >- (‘∃Δ₂. Δ' = {|A|} ⊎ Δ₂’
+        by (qexists_tac ‘Δ' - {|A|}’ >> irule SUB_BAG_DIFF_EQ >>
+            metis_tac[SUB_BAG_UNION_down]) >>
+      rw[] >> irule G_rc >> first_x_assum irule >> fs[])
+  >- (‘∃Δ₂. Δ' = BAG_INSERT (A And B) Δ₂’ 
+         by (qexists_tac ‘Δ' - {|A And B|}’ >> 
+             fs[BAG_INSERT_UNION] >> 
+             irule SUB_BAG_DIFF_EQ >> 
+             metis_tac[SUB_BAG_UNION_down]) >> 
+       rw[] >> irule G_rand >> fs[SUB_BAG_INSERT])
+  >- (‘∃Δ₂. Δ' = BAG_INSERT (A Or B) Δ₂’ 
+        by (qexists_tac ‘Δ' - {|A Or B|}’ >> 
+            fs[BAG_INSERT_UNION] >> 
+            irule SUB_BAG_DIFF_EQ >> 
+            metis_tac[SUB_BAG_UNION_down]) >>
+      rw[] >> fs[SUB_BAG_INSERT] >> irule G_rorl >> 
+      first_x_assum irule >> fs[SUB_BAG_INSERT])
+  >- (‘∃Δ₂. Δ' = BAG_INSERT (A Or B) Δ₂’ 
+        by (qexists_tac ‘Δ' - {|A Or B|}’ >> 
+            fs[BAG_INSERT_UNION] >> 
+            irule SUB_BAG_DIFF_EQ >> 
+            metis_tac[SUB_BAG_UNION_down]) >> 
+      rw[] >> fs[SUB_BAG_INSERT] >> irule G_rorr >> 
+      first_x_assum irule >> fs[SUB_BAG_INSERT])
+  >- (‘∃Δ₂. Δ' = BAG_INSERT (A Imp B) Δ₂’ 
+        by (qexists_tac ‘Δ' - {|A Imp B|}’ >> 
+            fs[BAG_INSERT_UNION] >> 
+            irule SUB_BAG_DIFF_EQ >> 
+            metis_tac[SUB_BAG_UNION_down]) >> 
+      rw[] >> fs[SUB_BAG_INSERT] >> irule G_limp >> conj_tac >>
+      first_x_assum (fn th => irule th >> fs[SUB_BAG_INSERT] >> NO_TAC))
+  >- (‘∃Δ₂. Δ' = BAG_INSERT (A Imp B) Δ₂’ 
+        by (qexists_tac ‘Δ' - {|A Imp B|}’ >> 
+            fs[BAG_INSERT_UNION] >> 
+            irule SUB_BAG_DIFF_EQ >> 
+            metis_tac[SUB_BAG_UNION_down]) >> 
+      rw[] >> fs[SUB_BAG_INSERT] >> irule G_rimp >> 
+      first_x_assum irule >> fs[SUB_BAG_INSERT])
+  >- (rename [‘Δ₁ ⊎ Δ₂ ≤ Δ₃’] >>
+      ‘∃Δ₀. Δ₃ = Δ₀ ⊎ Δ₁ ⊎ Δ₂’
+        by metis_tac[SUB_BAG_EXISTS, COMM_BAG_UNION, ASSOC_BAG_UNION] >>
+      fs[] >> rw[] >> irule G_cut >>
+      qexists_tac ‘A’ >> conj_tac >>
+      first_x_assum (fn th => irule th >> fs[SUB_BAG_INSERT] >> NO_TAC))
 QED
 
-val Gc_lc_AeA =
-    Q.prove(`∀A e Γ' B. (BAG_INSERT A (BAG_INSERT e (BAG_INSERT A Γ'))) Gc B
-            ==> (BAG_INSERT e (BAG_INSERT A Γ')) Gc B`,
+val G_lc_AeA =
+    Q.prove(`∀A e Γ'. G (BAG_INSERT A (BAG_INSERT e (BAG_INSERT A Γ'))) B
+            ==> G (BAG_INSERT e (BAG_INSERT A Γ')) B`,
             rw[] >>
-            `({|A;A|} ⊎ ({|e|} ⊎ Γ')) Gc B`
+            `G ({|A;A|} ⊎ ({|e|} ⊎ Γ')) B`
               by (fs[BAG_UNION_INSERT,ASSOC_BAG_UNION,BAG_INSERT_UNION] >>
                   simp[COMM_BAG_UNION] >>
                   fs[EL_BAG,BAG_UNION]) >>
-            `({|A|} ⊎ ({|e|} ⊎ Γ')) Gc B`
-              by metis_tac[Gc_lc] >>
-            `(({|A|} ⊎ {|e|}) ⊎ Γ') Gc B`
+            `G ({|A|} ⊎ ({|e|} ⊎ Γ')) B`
+              by metis_tac[G_lc] >>
+            `G (({|A|} ⊎ {|e|}) ⊎ Γ') B`
               by fs[ASSOC_BAG_UNION] >>
-            `(({|e|} ⊎ {|A|}) ⊎ Γ') Gc B`
+            `G (({|e|} ⊎ {|A|}) ⊎ Γ') B`
               by fs[COMM_BAG_UNION] >>
             fs[BAG_INSERT_UNION] >>
             fs[EL_BAG] >>
             simp[ASSOC_BAG_UNION]);
 
-Theorem Gc_INSERT_TO_MERGE:
-  ∀Γ. FINITE_BAG Γ ==> ∀A B. (BAG_INSERT A Γ) Gc B 
-      ==> (BAG_MERGE {|A|} Γ) Gc B
-Proof
-    Induct_on `Γ` >>
-    rw[] >>
-    Cases_on `A=e`
-        >- (fs[] >>
-            `BAG_MERGE {|e|} (BAG_INSERT e Γ) = BAG_INSERT e Γ`
-              by (simp[BAG_MERGE,BAG_INSERT,EMPTY_BAG,FUN_EQ_THM] >>
-                  rw[] >> fs[]) >>
-            fs[] >>
-            `({|e;e|} ⊎ Γ) Gc B` by fs[BAG_INSERT_UNION,ASSOC_BAG_UNION] >>
-            `({|e|} ⊎ Γ) Gc B` by metis_tac[Gc_lc] >>
-            `{|e|} ⊎ Γ = BAG_INSERT e Γ`
-              by rw[BAG_INSERT_UNION] >>
-            metis_tac[])
-        >- (Cases_on `BAG_IN A Γ`
-            >- (`?Γ'. Γ = BAG_INSERT A Γ'` by metis_tac[BAG_DECOMPOSE] >>
-                fs[] >>
-                `(BAG_INSERT e (BAG_INSERT A Γ')) Gc B`
-                  by metis_tac[Gc_lc_AeA] >>
-                fs[Gc_lw_BAG_MERGE])
-            >- (`BAG_INSERT A (BAG_INSERT e Γ)
-                 = BAG_MERGE {|A|} (BAG_INSERT e Γ)`
-                  by (`Γ A = 0` by metis_tac[NOT_BAG_IN] >>
-                      simp[BAG_INSERT,BAG_MERGE,EMPTY_BAG,FUN_EQ_THM] >>
-                      rw[] >>
-                      fs[COND_CLAUSES]) >>
-                fs[]))
-QED
-
 val unibag_AA_A = Q.prove(`unibag ({|A;A|} ⊎ Γ) = unibag ({|A|} ⊎ Γ)`,
   simp[unibag_thm]);
 
-Theorem Gc_unibag:
-  ∀Γ A. Γ Gc A <=> (unibag Γ) Gc A
+Theorem G_unibag:
+  ∀Γ A. G Γ A <=> G (unibag Γ) A
 Proof
   rw[] >> EQ_TAC
-  >- (`∀Γ. FINITE_BAG Γ ==> ∀A. Γ Gc A ==> (unibag Γ) Gc A`
-        suffices_by metis_tac[Gc_FINITE] >>
+  >- (`∀Γ. FINITE_BAG Γ ==> ∀A. G Γ A ==> G (unibag Γ) A`
+        suffices_by metis_tac[G_FINITE] >>
       gen_tac >>
       Induct_on `BAG_CARD Γ` >>
       rw[]
@@ -500,193 +448,144 @@ Proof
         >- (Cases_on `unibag Γ = Γ` >- fs[] >>
             drule_then strip_assume_tac unibag_DECOMPOSE >>
             rename [`Γ = {|B;B|} ⊎ Γ0`,`SUC n = BAG_CARD Γ`] >>
-            `({|B|} ⊎ Γ0) Gc A` by metis_tac[Gc_lc] >>
+            `G ({|B|} ⊎ Γ0) A` by metis_tac[G_lc] >>
             `BAG_CARD ({|B|} ⊎ Γ0) = n` by fs[BAG_CARD_THM] >>
             `FINITE_BAG ({|B|} ⊎ Γ0)` by fs[] >>
             metis_tac[unibag_AA_A]))
-   >- metis_tac[unibag_SUB_BAG,Gc_lw,Gc_FINITE,unibag_FINITE]
+   >- metis_tac[unibag_SUB_BAG,G_lw,G_FINITE,unibag_FINITE]
 QED
 
-Theorem Nc_Gc:
-  ∀Γ A. (Γ Nc A) ==> ((BAG_OF_SET Γ) Gc {|A|})
+Theorem N_G:
+  ∀D A. N D A ==> G (BAG_OF_SET D) A
 Proof
-  Induct_on `Γ Nc A` >>
-  rw[]
-  >- (irule Gc_ax >> simp[] >>
-      metis_tac[FINITE_BAG_OF_SET,FINITE_DEF])
-  >- (irule Gc_rand >> rw[]
-      >- (`(BAG_OF_SET (Γ' ∪ Γ)) Gc {|A|}`
-            suffices_by metis_tac[UNION_COMM] >>
-          simp[BAG_OF_SET_UNION] >>
-          metis_tac[Gc_lw_BAG_MERGE,Gc_FINITE])
-      >- (simp[BAG_OF_SET_UNION] >>
-              metis_tac[Gc_lw_BAG_MERGE,Gc_FINITE]))
-  >- (irule Gc_cut >>
-      qexists_tac `A And B` >>
-      conj_tac >- metis_tac[Gc_rw_BAG_INSERT,BAG_INSERT_commutes] >>
-      `{|A|} Gc {|A|}` by metis_tac[Gc_ax,BAG_IN_BAG_INSERT,FINITE_BAG] >>
-      `{|A And B|} Gc {|A|}` by metis_tac[Gc_landl] >>
-      simp[Once BAG_INSERT_UNION,EL_BAG] >>
-      irule Gc_lw_BAG_UNION >>
-      simp[] >>
-      metis_tac[Nc_FINITE])
-  >- (irule Gc_cut >>
-      qexists_tac `A And A'` >>
-      conj_tac >- metis_tac[Gc_rw_BAG_INSERT,BAG_INSERT_commutes] >>
-      `{|A'|} Gc {|A'|}` by metis_tac[Gc_ax,BAG_IN_BAG_INSERT,FINITE_BAG] >>
-      `{|A And A'|} Gc {|A'|}` by metis_tac[Gc_landr] >>
-      simp[Once BAG_INSERT_UNION,EL_BAG] >>
-      irule Gc_lw_BAG_UNION >>
-      simp[] >>
-      metis_tac[Nc_FINITE])
-  >- (irule Gc_rimp >>
-      fs[BAG_OF_SET_INSERT] >>
-      qexists_tac `A` >>
-      qexists_tac `A'` >>
-      irule Gc_lw >>
-      simp[] >>
-      drule Gc_FINITE >>
-      rw[] >>
-      qexists_tac `BAG_MERGE {|A|} (BAG_OF_SET Γ)` >>
-      simp[BAG_MERGE_ELBAG_SUB_BAG_INSERT] >>
-      `BAG_MERGE {|A|} (BAG_OF_SET Γ) Gc {|A Imp A';A'|}`
-        suffices_by metis_tac[BAG_INSERT_commutes] >>
-      metis_tac[Gc_rw_BAG_INSERT])
-  >- (rename [`Γ Nc A Imp B`] >>
-      simp[BAG_OF_SET_UNION] >>
-      (* `?b b'. (Γ = SET_OF_BAG b) ∧ (Γ' = SET_OF_BAG b')`  *)
-      (*   by (qexists_tac `BAG_OF_SET Γ` >> *)
-      (*       qexists_tac `BAG_OF_SET Γ'` >> *)
-      (*       rw[]) >> *)
-      (* fs[] >> rw[] > *)>
-      (* `unibag (b ⊎ b') Gc {|B|}` suffices_by metis_tac[unibag_UNION] >> *)
-      (* `b ⊎ b' Gc {|B|}` suffices_by metis_tac[Gc_unibag] >> *)
-      (* irule Gc_lcut >> *)
-      (* qexists_tac `A` >> *)
-      `FINITE_BAG (BAG_INSERT B (BAG_OF_SET Γ'))` 
-        by metis_tac[Nc_FINITE,FINITE_BAG_OF_SET,FINITE_BAG_INSERT] >>
-      `(BAG_INSERT B (BAG_OF_SET Γ')) Gc {|B|}` 
-        by (irule Gc_ax >> rw[]) >>
-      `(BAG_INSERT (A Imp B) (BAG_OF_SET Γ')) Gc {|B|}`
-        by metis_tac[Gc_limp,Gc_rw_BAG_INSERT,BAG_INSERT_commutes] >>
-      `((BAG_OF_SET Γ) ⊎ (BAG_OF_SET Γ')) Gc {|B|}`
-        by (irule Gc_cut >>
-            qexists_tac `A` >>
-            rw[]
-              >- (`BAG_OF_SET Γ' ⊎ BAG_OF_SET Γ Gc {|B;A|}`
-                    suffices_by metis_tac[COMM_BAG_UNION,BAG_INSERT_commutes] >>
-                  irule Gc_rw_BAG_INSERT >>
-                  irule Gc_lw_BAG_UNION >>
-                  conj_tac >- metis_tac[Gc_FINITE] >>
-                  simp[])
-              >- (
-                  qexists_tac `A` >>
-                  qexists_tac `B` >>
-                  qexists_tac `BAG_OF_SET Γ'` >>
-                  simp[]
-              
-
-  qabbrev_tac `Δ = ((BAG_OF_SET Γ) ⊎ (BAG_OF_SET Γ'))` >>
-      `FINITE_BAG (BAG_INSERT A' Δ)`
-        by (simp[Abbr`Δ`] >>
-            metis_tac[Nc_FINITE,FINITE_BAG_OF_SET,FINITE_BAG_UNION]) >>
-      `(BAG_INSERT A' Δ) Gc {|A'|}`
-        by metis_tac[Gc_ax,BAG_IN_BAG_INSERT,FINITE_BAG_THM] >>
-      `(BAG_INSERT A' Δ) Gc {|A;A'|}`
-        by metis_tac[Gc_rw_BAG_INSERT] >>
-      `Δ Gc {|A;A'|}`
-        by (simp[Abbr`Δ`] >>
-            `BAG_OF_SET Γ' ⊎ BAG_OF_SET Γ Gc {|A';A|}`
-             suffices_by metis_tac[COMM_BAG_UNION,BAG_INSERT_commutes]
-            irule Gc_lw_BAG_UNION >>
+ Induct_on `N` >>
+ rw[G_rules]
+ (* >- (irule G_ax >> simp[] >> *)
+ (*     metis_tac[FINITE_BAG_OF_SET,FINITE_DEF]) *)
+ >- (irule G_rand >> conj_tac
+     >- (`G (BAG_OF_SET (D' ∪ D)) A` suffices_by metis_tac[UNION_COMM] >>
+         simp[BAG_OF_SET_UNION] >>
+         metis_tac[G_lw_BAG_MERGE,G_FINITE])
+     >- (simp[BAG_OF_SET_UNION] >>
+             metis_tac[G_lw_BAG_MERGE,G_FINITE]))
+ >- (`G {|A|} A` by metis_tac[G_ax,BAG_IN_BAG_INSERT,FINITE_BAG] >>
+     `G {|A And B|} A` by metis_tac[G_landl] >>
+     `G ((BAG_OF_SET D) + {||}) A` by metis_tac[G_cut] >>
+     metis_tac[BAG_UNION_EMPTY])
+ >- (`G {|A'|} A'` by metis_tac[G_ax,BAG_IN_BAG_INSERT,FINITE_BAG] >>
+     `G {|A And A'|} A'` by metis_tac[G_landr] >>
+     `G ((BAG_OF_SET D) + {||}) A'` by metis_tac[G_cut] >>
+     metis_tac[BAG_UNION_EMPTY])
+ >- (irule G_rimp >>
+     fs[BAG_OF_SET_INSERT] >>
+     irule G_lw >>
+     simp[] >>
+     drule G_FINITE >>
+     rw[] >>
+     qexists_tac `BAG_MERGE {|A|} (BAG_OF_SET D)` >>
+     simp[BAG_MERGE_ELBAG_SUB_BAG_INSERT])
+ >- (simp[BAG_OF_SET_UNION] >>
+    `FINITE_BAG (BAG_OF_SET D')` by metis_tac[N_FINITE,FINITE_BAG_OF_SET] >>
+    `G (BAG_INSERT A' (BAG_OF_SET D')) A'`
+      by simp[G_ax,BAG_IN_BAG_INSERT] >>
+    `G (BAG_INSERT (A Imp A') (BAG_OF_SET D')) A'`
+      by metis_tac[G_limp] >>
+    `G ((BAG_OF_SET D) ⊎ (BAG_OF_SET D')) A'`
+      by metis_tac[G_cut] >>
+    `G (unibag (BAG_OF_SET D ⊎ BAG_OF_SET D')) A'` by metis_tac[G_unibag] >>
+    fs[unibag_UNION])
+ >- (rename [`N (_ INSERT _) C`] >>
+     fs[BAG_OF_SET_UNION,BAG_OF_SET_INSERT] >>
+     qabbrev_tac `Δ = ((BAG_OF_SET D) ⊎ (BAG_OF_SET D1) ⊎ (BAG_OF_SET D2))` >>
+     `FINITE_BAG (BAG_INSERT A Δ)`
+       by (simp[Abbr`Δ`,FINITE_BAG_THM] >>
+           metis_tac[FINITE_BAG_OF_SET,N_FINITE,FINITE_INSERT]) >>
+      `G (BAG_INSERT A Δ) C`
+        by (`G (BAG_MERGE {|A|} Δ) C`
+              suffices_by metis_tac[BAG_MERGE_ELBAG_SUB_BAG_INSERT,G_lw] >>
+            simp[Abbr`Δ`] >>
+            irule G_lw >>
+            conj_tac >- fs[FINITE_BAG_MERGE,FINITE_BAG_THM] >>
+            qexists_tac `BAG_MERGE {|A|} (BAG_OF_SET D1)` >>
             simp[] >>
-            conj_tac >- metis_tac[Nc_FINITE] >>
-            metis_tac[Gc_rw_BAG_INSERT]) >>
-      `(BAG_INSERT (A Imp A') Δ) Gc {|A'|}`
-        by metis_tac[Gc_limp] >>
-      `Δ Gc {|A Imp A'|}`
+            fs[BAG_MERGE,BAG_INSERT,EMPTY_BAG,
+               BAG_OF_SET,BAG_UNION,SUB_BAG,BAG_INN,IN_DEF] >>
+            rw[] >>
+            fs[]) >>
+      `FINITE_BAG (BAG_INSERT B Δ)`
+      by (simp[Abbr`Δ`,FINITE_BAG_THM] >>
+              metis_tac[FINITE_BAG_OF_SET,N_FINITE,FINITE_INSERT]) >>
+      `G (BAG_INSERT B Δ) C`
+        by (`G (BAG_MERGE {|B|} Δ) C`
+              suffices_by metis_tac[BAG_MERGE_ELBAG_SUB_BAG_INSERT,G_lw] >>
+            simp[Abbr`Δ`] >>
+            irule G_lw >>
+            conj_tac >- fs[FINITE_BAG_MERGE,FINITE_BAG_THM] >>
+            qexists_tac `BAG_MERGE {|B|} (BAG_OF_SET D2)` >>
+            simp[] >>
+            fs[BAG_MERGE,BAG_INSERT,EMPTY_BAG,
+               BAG_OF_SET,BAG_UNION,SUB_BAG,BAG_INN,IN_DEF] >>
+            rw[] >>
+            fs[]) >>
+      `G Δ (A Or B)`
         by (simp[Abbr`Δ`] >>
-            metis_tac[Gc_lw_BAG_UNION,Gc_FINITE]) >>
-      
-      `Δ Gc {|A'|}`
-        by metis_tac[Gc_cut] >>
-      `(unibag (BAG_OF_SET Γ ⊎ BAG_OF_SET Γ')) Gc {|A'|}` by metis_tac[Gc_unibag] >>
-      fs[unibag_UNION])
-  >- (rename [`Nc (_ INSERT _) C`] >>
-      fs[BAG_OF_SET_UNION,BAG_OF_SET_INSERT] >>
-      qabbrev_tac `Δ = ((BAG_OF_SET Γ) ⊎ (BAG_OF_SET D1) ⊎ (BAG_OF_SET D2))` >>
-      `FINITE_BAG (BAG_INSERT A Δ)`
-        by (simp[Abbr`Δ`,FINITE_BAG_THM] >>
-            metis_tac[FINITE_BAG_OF_SET,Nc_FINITE,FINITE_INSERT]) >>
-        `Gc (BAG_INSERT A Δ) C`
-          by (`Gc (BAG_MERGE {|A|} Δ) C`
-                suffices_by metis_tac[BAG_MERGE_ELBAG_SUB_BAG_INSERT,Gc_lw] >>
-              simp[Abbr`Δ`] >>
-              irule Gc_lw >>
-              conj_tac >- fs[FINITE_BAG_MERGE,FINITE_BAG_THM] >>
-              qexists_tac `BAG_MERGE {|A|} (BAG_OF_SET D1)` >>
-              simp[] >>
-              fs[BAG_MERGE,BAG_INSERT,EMPTY_BAG,
-                BAG_OF_SET,BAG_UNION,SUB_BAG,BAG_INN,IN_DEF] >>
-              rw[] >>
-              fs[]) >>
-        `FINITE_BAG (BAG_INSERT B Δ)`
-        by (simp[Abbr`Δ`,FINITE_BAG_THM] >>
-                metis_tac[FINITE_BAG_OF_SET,Nc_FINITE,FINITE_INSERT]) >>
-        `Gc (BAG_INSERT B Δ) C`
-          by (`Gc (BAG_MERGE {|B|} Δ) C`
-                suffices_by metis_tac[BAG_MERGE_ELBAG_SUB_BAG_INSERT,Gc_lw] >>
-              simp[Abbr`Δ`] >>
-              irule Gc_lw >>
-              conj_tac >- fs[FINITE_BAG_MERGE,FINITE_BAG_THM] >>
-              qexists_tac `BAG_MERGE {|B|} (BAG_OF_SET D2)` >>
-              simp[] >>
-              fs[BAG_MERGE,BAG_INSERT,EMPTY_BAG,
-                BAG_OF_SET,BAG_UNION,SUB_BAG,BAG_INN,IN_DEF] >>
-              rw[] >>
-              fs[]) >>
-        `Gc Δ (A Or B)`
-          by (simp[Abbr`Δ`] >>
-              irule Gc_lw_BAG_UNION >>
-              conj_tac >- metis_tac[FINITE_INSERT,Nc_FINITE,FINITE_BAG_OF_SET] >>
-              irule Gc_lw_BAG_UNION >>
-              conj_tac >- metis_tac[FINITE_INSERT,Nc_FINITE,FINITE_BAG_OF_SET] >>
-              metis_tac[]) >>
-        `Gc (BAG_INSERT (A Or B) Δ) C` by metis_tac[Gc_lor] >>
-        `Gc ((BAG_OF_SET Γ) ⊎ Δ) C` by metis_tac[Gc_cut] >>
-        `Gc (unibag (BAG_OF_SET Γ ⊎ Δ)) C` by metis_tac[Gc_unibag] >>
-        `(unibag (BAG_OF_SET Γ ⊎ Δ))
-          = BAG_MERGE (BAG_MERGE (BAG_OF_SET Γ) (BAG_OF_SET D1)) (BAG_OF_SET D2)`
-          suffices_by metis_tac[] >>
-        rw[Abbr`Δ`,unibag_UNION,BAG_MERGE,FUN_EQ_THM])
-  >- (`Gc {|Bot|} A` by metis_tac[Gc_bot,BAG_IN_BAG_INSERT,FINITE_BAG] >>
-      metis_tac[Gc_cut,BAG_UNION_EMPTY])
- );
+            irule G_lw_BAG_UNION >>
+            conj_tac >- metis_tac[FINITE_INSERT,N_FINITE,FINITE_BAG_OF_SET] >>
+            irule G_lw_BAG_UNION >>
+            conj_tac >- metis_tac[FINITE_INSERT,N_FINITE,FINITE_BAG_OF_SET] >>
+            metis_tac[]) >>
+      `G (BAG_INSERT (A Or B) Δ) C` by metis_tac[G_lor] >>
+      `G ((BAG_OF_SET D) ⊎ Δ) C` by metis_tac[G_cut] >>
+      `G (unibag (BAG_OF_SET D ⊎ Δ)) C` by metis_tac[G_unibag] >>
+      `(unibag (BAG_OF_SET D ⊎ Δ))
+        = BAG_MERGE (BAG_MERGE (BAG_OF_SET D) (BAG_OF_SET D1)) (BAG_OF_SET D2)`
+         suffices_by metis_tac[] >>
+      rw[Abbr`Δ`,unibag_UNION,BAG_MERGE,FUN_EQ_THM])
+ >- (`G {|Bot|} A` by metis_tac[G_bot,BAG_IN_BAG_INSERT,FINITE_BAG] >>
+     metis_tac[G_cut,BAG_UNION_EMPTY])
+QED
 
-(* Apparently Nc takes a subset here!? *)
-Theorem Gc_Nc `∀Γ A. Gc Γ A ==> ?Γ'. Γ' ⊆ (SET_OF_BAG Γ) /\ Nc Γ' A` (
-  Induct_on `Gc` >> rw[]
-    >- (qexists_tac `{A}` >> simp[SUBSET_DEF,SET_OF_BAG] >> metis_tac[Nc_ax])
-    >- (qexists_tac `{Bot}` >> simp[SUBSET_DEF,SET_OF_BAG] >>
-        metis_tac[Nc_bot,Nc_ax])
-    >- (qexists_tac `Γ'` >> fs[SET_OF_BAG,BAG_UNION,BAG_INSERT])
-    >- (rename [`Nc _ C`] >>
-        `Nc {A And B} (A And B)` by metis_tac[Nc_ax] >>
-        `Nc {A And B} A` by metis_tac[Nc_andel] >>
-        `Nc (Γ' DELETE A) (A Imp C)`
-          by metis_tac[Nc_impi_DELETE] >>
-        `Nc ((Γ' DELETE A) ∪ {A And B}) C` by metis_tac[Nc_impe] >>
-        `Nc ((A And B) INSERT (Γ' DELETE A)) C`
-                  by metis_tac[UNION_COMM,INSERT_SING_UNION] >>
-        qexists_tac `(A And B) INSERT Γ' DELETE A` >>
+Theorem G_N:
+  ∀Γ A. G Γ A ==> N (SET_OF_BAG Γ) A
+Proof
+  Induct_on `G` >> rw[N_rules]
+    >- (`?b. Γ = BAG_INSERT A b` by metis_tac[BAG_DECOMPOSE] >>
+        fs[] >> 
+        simp[SET_OF_BAG_INSERT, Once INSERT_SING_UNION] >>
+        `N {A} A` by metis_tac[N_ax] >>
+        simp[UNION_COMM] >>
+        irule N_lw_SUBSET >>
+        conj_tac >- metis_tac[FINITE_UNION,FINITE_SET_OF_BAG,FINITE_DEF] >>
+        metis_tac[SUBSET_UNION])
+    >- (`?b. Γ = BAG_INSERT Bot b` by metis_tac[BAG_DECOMPOSE] >>
+        fs[] >> 
+        simp[SET_OF_BAG_INSERT, Once INSERT_SING_UNION] >>
+        `N {Bot} Bot` by metis_tac[N_ax] >>
+        `N {Bot} A` by metis_tac[N_bot] >>
+        irule N_lw_SUBSET >>
+        conj_tac >- metis_tac[FINITE_UNION,FINITE_SET_OF_BAG,FINITE_DEF] >>
+        metis_tac[SUBSET_UNION])
+    >- fs[SET_OF_BAG,BAG_UNION,BAG_INSERT]
+    >- (rename [`N _ C`] >>
         fs[SET_OF_BAG_INSERT] >>
-        fs[SUBSET_DEF] >>
-        metis_tac[])
-    >- (rename [`Nc _ C`] >>
-        `Nc {A And B} (A And B)` by metis_tac[Nc_ax] >>
-        `Nc {A And B} B` by metis_tac[Nc_ander] >>
-        `Nc (B INSERT Γ') C` by metis_tac[Nc_lw] >>
-        `Nc (Γ' DELETE B) (B Imp C)`
+        `N {A And B} (A And B)` by metis_tac[N_ax] >>
+        `N {A And B} A` by metis_tac[N_andel] >>
+        `N ((A INSERT (SET_OF_BAG Γ)) DELETE A) (A Imp C)`
+          by metis_tac[N_impi_DELETE] >>
+        fs[DELETE_DEF] >>
+        `N (((SET_OF_BAG Γ) DIFF {A}) ∪ {A And B}) C` by metis_tac[N_impe] >>
+        `N ((A And B) INSERT ((SET_OF_BAG Γ) DIFF {A})) C`
+                  by metis_tac[UNION_COMM,INSERT_SING_UNION] >>
+        irule N_lw_SUBSET >>
+        conj_tac >- metis_tac[N_FINITE,FINITE_INSERT] >>
+        qexists_tac `(A And B) INSERT SET_OF_BAG Γ DIFF {A}` >>
+        rw[SUBSET_DEF])
+    >- (rename [`N _ C`] >>
+        `N {A And B} (A And B)` by metis_tac[N_ax] >>
+        `N {A And B} B` by metis_tac[N_ander] >>
+        qabbrev_tac `Γ'= SET_OF_BAG (BAG_INSERT B Γ)` >>
+        `N (B INSERT Γ') C` by metis_tac[N_lw] >>
+        `N (Γ' DELETE B) (B Imp C)`
           by (Cases_on `B ∈ Γ'`
               >- (`?Γ0. (Γ' = B INSERT Γ0) /\ B NOTIN Γ0`
                     by metis_tac[DECOMPOSITION] >>
@@ -694,96 +593,97 @@ Theorem Gc_Nc `∀Γ A. Gc Γ A ==> ?Γ'. Γ' ⊆ (SET_OF_BAG Γ) /\ Nc Γ' A` (
                   `(B INSERT Γ0) DELETE B = Γ0`
                     by (dsimp[EXTENSION] >>
                         metis_tac[]) >>
-                  simp[Nc_impi])
-              >- (simp[DELETE_NON_ELEMENT_RWT,Nc_impi])) >>
-        `Nc ((Γ' DELETE B) ∪ {A And B}) C` by metis_tac[Nc_impe] >>
-        `Nc ((A And B) INSERT (Γ' DELETE B)) C`
+                  simp[N_impi])
+              >- (simp[DELETE_NON_ELEMENT_RWT,N_impi])) >>
+        `N ((Γ' DELETE B) ∪ {A And B}) C` by metis_tac[N_impe] >>
+        `N ((A And B) INSERT (Γ' DELETE B)) C`
           by metis_tac[UNION_COMM,INSERT_SING_UNION] >>
-        qexists_tac `(A And B) INSERT Γ' DELETE B` >>
-        fs[SET_OF_BAG_INSERT] >>
-        fs[SUBSET_DEF] >>
-        metis_tac[])
-    >- (qexists_tac `Γ' ∪ Γ''` >> simp[] >>
-        metis_tac[Nc_andi])
-    >- (rename [`Nc _ C`] >>
+        fs[Abbr`Γ'`,SET_OF_BAG_INSERT] >>
+        irule N_lw_SUBSET >>
+        conj_tac >- metis_tac[N_FINITE,FINITE_INSERT] >>
+        fs[DELETE_DEF] >>
+        qexists_tac `(A And B) INSERT SET_OF_BAG Γ DIFF {B}` >>
+        rw[SUBSET_DEF])
+    >- (rename [`N _ (A And B)`] >> metis_tac[N_andi,UNION_IDEMPOT])
+    >- (rename [`N _ C`] >>
         qabbrev_tac `Δ = (A Or B) INSERT (SET_OF_BAG Γ)` >>
+        qabbrev_tac `Γ' = A INSERT (SET_OF_BAG Γ)` >>
+        qabbrev_tac `Γ'' = B INSERT (SET_OF_BAG Γ)` >>
         fs[SET_OF_BAG_INSERT] >>
-        `FINITE_BAG Γ` by metis_tac[Gc_FINITE,FINITE_BAG_THM] >>
-        `Nc (A INSERT Δ) C`
-          by (irule Nc_lw_SUBSET >>
+        `FINITE_BAG Γ` by metis_tac[G_FINITE,FINITE_BAG_THM] >>
+        `N (A INSERT Δ) C`
+          by (irule N_lw_SUBSET >>
               simp[Abbr`Δ`] >>
               qexists_tac `Γ'` >>
-              simp[] >>
-              metis_tac[INSERT_COMM,SUBSET_INSERT_RIGHT]) >>
-        `Nc (B INSERT Δ) C`
-          by (irule Nc_lw_SUBSET >>
+              simp[Abbr`Γ'`,SUBSET_INSERT_RIGHT]) >>
+        `N (B INSERT Δ) C`
+          by (irule N_lw_SUBSET >>
               simp[Abbr`Δ`] >>
               qexists_tac `Γ''` >>
-              simp[] >>
-              metis_tac[INSERT_COMM,SUBSET_INSERT_RIGHT]) >>
-        qexists_tac `Δ` >>
-        simp[] >>
-        `Nc {(A Or B)} (A Or B)` by metis_tac[Nc_ax] >>
+              simp[Abbr`Γ''`,SUBSET_INSERT_RIGHT]) >>
+        `N {(A Or B)} (A Or B)` by metis_tac[N_ax] >>
         `FINITE ({A Or B} ∪ (SET_OF_BAG Γ))`
           by (`FINITE (SET_OF_BAG Γ)`
                 by metis_tac[FINITE_SET_OF_BAG] >>
               metis_tac[FINITE_UNION,FINITE_DEF]) >>
-        `Nc ({A Or B} ∪ (SET_OF_BAG Γ)) (A Or B)`
-          by metis_tac[SUBSET_UNION,Nc_lw_SUBSET] >>
-        `Nc Δ (A Or B)`
-          by (simp[Abbr`Δ`] >>metis_tac[INSERT_SING_UNION]) >>
-        `Nc (Δ ∪ Δ ∪ Δ) C` by metis_tac[Nc_ore] >>
+        `N ({A Or B} ∪ (SET_OF_BAG Γ)) (A Or B)`
+          by metis_tac[SUBSET_UNION,N_lw_SUBSET] >>
+        `N Δ (A Or B)`
+          by (simp[Abbr`Δ`,Abbr`Γ'`,Abbr`Γ''`] >>
+              irule N_lw_SUBSET >>
+              rw[] >>
+              qexists_tac `{A Or B}` >>
+              simp[]) >>
+        `N (Δ ∪ Δ ∪ Δ) C` by metis_tac[N_ore] >>
         metis_tac[UNION_IDEMPOT])
-    >- (qexists_tac `Γ'` >> simp[Nc_orir])
-    >- (qexists_tac `Γ'` >> simp[Nc_oril])
-    >- (rename [`Nc _ C`] >>
+    >- (rename [`N _ C`] >>
         fs[SET_OF_BAG_INSERT] >>
-        `FINITE_BAG Γ` by metis_tac[Gc_FINITE,FINITE_BAG_THM] >>
+        `FINITE_BAG Γ` by metis_tac[G_FINITE,FINITE_BAG_THM] >>
         `FINITE (SET_OF_BAG Γ)` by metis_tac[FINITE_SET_OF_BAG] >>
-        `Nc {A Imp B} (A Imp B)` by metis_tac[Nc_ax] >>
-        `Nc (SET_OF_BAG Γ) A` by metis_tac[Nc_lw_SUBSET] >>
-        `Nc ({A Imp B} ∪ (SET_OF_BAG Γ)) B` by metis_tac[Nc_impe] >>
-        `Nc ((A Imp B) INSERT (SET_OF_BAG Γ)) B`
-          by metis_tac[INSERT_SING_UNION] >>
-        qexists_tac `(A Imp B) INSERT SET_OF_BAG Γ` >>
-        simp[SUBSET_INSERT_RIGHT] >>
-        `Nc (B INSERT (SET_OF_BAG Γ)) C`
-          by metis_tac[Nc_lw_SUBSET,FINITE_INSERT] >>
-        `Nc (SET_OF_BAG Γ) (B Imp C)` by metis_tac[Nc_impi] >>
-        `Nc ((SET_OF_BAG Γ) ∪ ((A Imp B) INSERT SET_OF_BAG Γ)) C`
-          by metis_tac[Nc_impe] >>
-        metis_tac[UNION_COMM,UNION_ASSOC,UNION_IDEMPOT,INSERT_SING_UNION])
-    >- (rename [`Nc Δ C`,`Nc _ (A Imp C)`] >>
+        `N {A Imp B} (A Imp B)` by metis_tac[N_ax] >>
+        `N ((A Imp B) INSERT (SET_OF_BAG Γ)) B`
+          by metis_tac[INSERT_SING_UNION,N_impe] >>
+        irule N_lw_SUBSET >>
+        rw[] >>
+        `N (B INSERT (SET_OF_BAG Γ)) C`
+          by metis_tac[N_lw_SUBSET,FINITE_INSERT] >>
+        `N (SET_OF_BAG Γ) (B Imp C)` by metis_tac[N_impi] >>
+        `N ((SET_OF_BAG Γ) ∪ ((A Imp B) INSERT SET_OF_BAG Γ)) C`
+          by metis_tac[N_impe] >>
+        `N ((A Imp B) INSERT SET_OF_BAG Γ) C`
+          by metis_tac[UNION_COMM,UNION_ASSOC,UNION_IDEMPOT,INSERT_SING_UNION]>>
+        qexists_tac `(A Imp B) INSERT (SET_OF_BAG Γ)` >>
+        rw[] >>
+        fs[SUBSET_INSERT_RIGHT])
+    >- (rename [`N _ (A Imp C)`] >>
         fs[SET_OF_BAG_INSERT] >>
-        `FINITE (A INSERT (SET_OF_BAG Γ))`
-          by (simp[] >> metis_tac[Gc_FINITE,FINITE_BAG_THM]) >>
-        `Nc (A INSERT (SET_OF_BAG Γ)) C` by metis_tac[Nc_lw_SUBSET] >>
-        `Nc (SET_OF_BAG Γ) (A Imp C)` by metis_tac[Nc_impi] >>
-        metis_tac[SUBSET_REFL])
-    >- (rename [`Gc Γ A`,`Gc (BAG_INSERT A Γ2) B`,`Nc Δ1 A`,`Nc Δ2 B`] >>
-        `Nc (A INSERT Δ2) B` by metis_tac[Nc_lw] >>
-        `Nc (Δ2 DELETE A) (A Imp B)` by metis_tac[Nc_impi_DELETE] >>
-        `Nc ((Δ2 DELETE A) ∪ Δ1) B` by metis_tac[Nc_impe] >>
-        qexists_tac `((Δ2 DELETE A) ∪ Δ1)` >>
-        rw[]
-          >- (irule SUBSET_TRANS >>
-              qexists_tac `(SET_OF_BAG Γ2)` >>
-              fs[SET_OF_BAG_INSERT,SET_OF_BAG_UNION] >>
-              fs[SUBSET_DEF] >>
-              metis_tac[])
-          >- (fs[SET_OF_BAG_UNION] >>
-              metis_tac[SUBSET_DEF,IN_UNION])
-));
+        metis_tac[N_impi])
+    >- (rename [`G (BAG_INSERT A Δ) B`] >>
+        fs[SET_OF_BAG_INSERT] >>
+        `N ((A INSERT SET_OF_BAG Δ) DELETE A) (A Imp B)`
+          by metis_tac[N_impi_DELETE] >>
+        fs[DELETE_DEF] >>
+        `N ((SET_OF_BAG Δ DIFF {A}) ∪ (SET_OF_BAG Γ)) B` by metis_tac[N_impe] >>
+        irule N_lw_SUBSET >>
+        reverse(rw[])
+          >- (qexists_tac `SET_OF_BAG Δ DIFF {A} ∪ SET_OF_BAG Γ` >>
+              rw[]
+              >- (irule SUBSET_TRANS >>
+                  qexists_tac `(SET_OF_BAG Δ)` >>
+                  fs[SET_OF_BAG_INSERT,SET_OF_BAG_UNION])
+              >- fs[SET_OF_BAG_UNION])
+          >> metis_tac[G_FINITE,FINITE_BAG_THM])
+QED
 
-Theorem Gc_iff_Nc
-`∀Γ A. Gc Γ A <=> Nc (SET_OF_BAG Γ) A` (
+Theorem G_iff_N:
+∀Γ A. G Γ A <=> N (SET_OF_BAG Γ) A
+Proof
+  rw[G_N] >>
+  EQ_TAC >- rw[G_N] >>
   rw[] >>
-  EQ_TAC
-    >- (rw[] >>
-      `?D. D ⊆ (SET_OF_BAG Γ) ∧ Nc D A` by metis_tac[Gc_Nc] >>
-      metis_tac[Nc_lw_SUBSET,Gc_FINITE,FINITE_SET_OF_BAG]) >>
-  rw[] >>
-  `Gc (unibag Γ) A` by metis_tac[Nc_Gc] >>
-  metis_tac[Gc_unibag]);
+  `G (unibag Γ) A` by metis_tac[N_G] >>
+  metis_tac[G_unibag]
+QED
+
 
 val _ = export_theory()
